\section{Potential}

Consider
$$
F_t(x) = \exp\left( f_t(x) \right) \; .
$$
where $f_t(x) = \sum_{n=1}^\infty a_{2n} x^{2n}$ and where $a_2 > 0$ and $a_4,
a_6 \dots, \ge 0$. Then $f_t$ is even, strictly convex and satisfies $x \cdot
f_t''(x) \ge f_t'(x)$. Consequently, $F_t(x)$ is even, logarithmically convex,
and satisfies $x\cdot F_t''(x) \ge F_t'(x)$.

We need to define prediction fraction $b_t$ and verify that
$$
(1 + z_t b_t) F_t(x_{t-1}) \ge F_{t+1}(z_t + x_{t-1}) \; .
$$
Taking logarithm, this is equivalent to
$$
f_t(x_{t-1}) \ge f_{t+1}(z_t + x_{t-1}) - \ln(1 + z_t b_t) \; .
$$
Let $\phi_t(z) = f_{t+1}(z + x_{t-1}) - \ln (1 + z b_t)$ be right hand side of the inequality.
Since $\phi_t(z)$ is convex, we have
$$
\phi_t(z) \le \max\{ \phi_t(1), \phi_t(-1) \} \; .
$$
We define $b_t$ so that $\phi_t(1) = \phi(-1)$, which is equivalent to
$$
f_{t+1}(x_{t-1} + 1) - \ln (1 + b_t) = f_{t+1}(x_{t-1} - 1) - \ln (1 - b_t) \; .
$$
Taking $\exp()$ of both sides, gives
$$
\frac{F_{t+1}(x_{t-1} + 1)}{1 + b_t} = \frac{F_{t+1}(x_{t-1} - 1)}{1 - b_t} \; .
$$
Solving for $b_t$ gives
$$
b_t  =  \frac{F_{t+1}(x_{t-1} + 1) - F_{t+1}(x_{t-1} - 1)}{F_{t+1}(x_{t-1} - 1) + F_{t+1}(x_{t-1} + 1)} \; .
$$
With this choice of $b_t$, we have
\begin{align*}
\phi_t(0) = \phi_t(1)
& = f_{t+1}(x_{t-1} + 1) - \ln (1 + b_t) \\
& = f_{t+1}(x_{t-1} + 1) - \ln\left(1 + \frac{F_{t+1}(x_{t-1} + 1) - F_{t+1}(x_{t-1} - 1)}{F_{t+1}(x_{t-1} - 1) + F_{t+1}(x_{t-1} + 1)}\right) \\
& = f_{t+1}(x_{t-1} + 1) - \ln\left(\frac{2 F_{t+1}(x_{t-1} + 1)}{F_{t+1}(x_{t-1} - 1) + F_{t+1}(x_{t-1} + 1)}\right) \\
& = f_{t+1}(x_{t-1} + 1) - \ln(2) - f_{t+1}(x_{t-1} + 1) + \ln \left(F_{t+1}(x_{t-1} - 1) + F_{t+1}(x_{t-1} + 1)\right) \\
& = - \ln(2) + \ln \left(F_{t+1}(x_{t-1} - 1) + F_{t+1}(x_{t-1} + 1)\right) \\
& =  \ln \left( \frac{F_{t+1}(x_{t-1} - 1) + F_{t+1}(x_{t-1} + 1)}{2}\right) \; .
\end{align*}
Thus, it remains to prove that
$$
f_t(x_{t-1}) \ge \ln \left( \frac{F_{t+1}(x_{t-1} - 1) + F_{t+1}(x_{t-1} + 1)}{2}\right)
$$
Which is equivalent to
$$
F_t(x_{t-1}) \ge \frac{F_{t+1}(x_{t-1} - 1) + F_{t+1}(x_{t-1} + 1)}{2} \; .
$$

\subsection{Gamma Potential}

We consider
$$
F_t(x) = \frac{2^{t-1} \Gamma(\frac{t+1}{2} + \frac{x}{2})\Gamma(\frac{t+1}{2} - \frac{x}{2})}{\pi t!} \; .
$$
The inequality
\begin{align*}
\frac{F_{t+1}(x_{t-1} - 1) + F_{t+1}(x_{t-1} + 1)}{2}
& = \frac{2^t \Gamma(\frac{t+2}{2} + \frac{x-1}{2})\Gamma(\frac{t+2}{2} - \frac{x-1}{2})}{2\pi (t+1)!} + \frac{2^t \Gamma(\frac{t+2}{2} + \frac{x+1}{2})\Gamma(\frac{t+2}{2} - \frac{x+1}{2})}{2\pi (t+1)!} \\
& = \frac{2^t \Gamma(\frac{t+1}{2} + \frac{x}{2})\Gamma(\frac{t+3}{2} - \frac{x}{2})}{2\pi (t+1)!} + \frac{2^t \Gamma(\frac{t+3}{2} + \frac{x}{2})\Gamma(\frac{t+1}{2} - \frac{x}{2})}{2\pi (t+1)!} \\
& = \frac{2^t \Gamma(\frac{t+1}{2} + \frac{x}{2})\Gamma(\frac{t+1}{2} - \frac{x}{2})(\frac{t+1}{2} - \frac{x}{2})}{2\pi (t+1)!} + \frac{2^t (\frac{t+1}{2} + \frac{x}{2})\Gamma(\frac{t+1}{2} + \frac{x}{2})\Gamma(\frac{t+1}{2} - \frac{x}{2})}{2\pi (t+1)!} \\
& = \left( \frac{t+1}{2} - \frac{x}{2} + \frac{t+1}{2} + \frac{x}{2} \right) \frac{2^t \Gamma(\frac{t+1}{2} + \frac{x}{2})\Gamma(\frac{t+1}{2} - \frac{x}{2})}{2\pi (t+1)!} \\
& = 2^{t-1} \frac{\Gamma(\frac{t+1}{2} + \frac{x}{2})\Gamma(\frac{t+1}{2} - \frac{x}{2})}{\pi t!} \\
& = F_t(x_{t-1}) \\
\end{align*}


\subsection{Concrete Example 2}

We consider
$$
F_t(x) = \exp\left( \frac{x^2}{2t} - \ln\left(2 - \frac{1}{t} \right) \right) \; .
$$
The inequality
